src/lowparse/LowParse.Steel.Combinators.fst
@@ -7,9 +7,10 @@ include LowParse.Spec.Combinators
 module S = Steel.Memory
 module SE = Steel.Effect
 module SEA = Steel.Effect.Atomic
-module A = Steel.Array
+module A = Steel.C.Array
 module AP = LowParse.Steel.ArrayPtr
 
+module SZ = Steel.C.StdInt
 module U32 = FStar.UInt32
 module U64 = FStar.UInt64
 
@@ -27,11 +28,11 @@ let validate_pair
 : Pure (wvalidator (p1 `nondep_then` p2))
   (requires (k1.parser_kind_subkind == Some ParserStrong))
   (ensures (fun _ -> True))
-= fun a len ->
-  let ga : Ghost.erased (AP.v byte) = SEA.gget (AP.varrayptr a) in
+= fun base a len ->
+  let ga : Ghost.erased (AP.v base byte) = SEA.gget (AP.varrayptr a) in
   let g : Ghost.erased _ = ga.AP.contents in
   nondep_then_eq p1 p2 g;
-  let r1 = v1 a len in
+  let r1 = v1 base a len in
   if is_error r1
   then begin
     SEA.return r1
@@ -39,14 +40,12 @@ let validate_pair
   else begin
     let sq : squash (is_success r1) = () in // FIXME: WHY WHY WHY does refinement or requires not work?
     let consumed = uint64_to_uint32 r1 sq in
-    let a2 = AP.split a consumed in
-    SEA.reveal_star (AP.varrayptr a) (AP.varrayptr a2); // FIXME: WHY WHY WHY is this needed?
-    let ga1 : Ghost.erased (AP.v byte) = SEA.gget (AP.varrayptr a) in
+    let a2 = AP.split a (SZ.mk_size_t consumed) in
+    let ga1 : Ghost.erased (AP.v base byte) = SEA.gget (AP.varrayptr a) in
     let g1 : Ghost.erased _ = ga1.AP.contents in
     parse_strong_prefix p1 g1 g;
-    let ga2 : Ghost.erased (AP.v byte) = SEA.gget (AP.varrayptr a2) in // FIXME: WHY WHY WHY is this needed?
     let len2 = len `U32.sub` consumed in
-    let r2 = v2 a2 len2 in
+    let r2 = v2 base a2 len2 in
     AP.join a a2;
     if is_error r2
     then SEA.return r2
@@ -67,8 +66,9 @@ val destruct_pair
   (#k2: parser_kind)
   (#t2: Type)
   (p2: parser k2 t2)
-  (a: byte_array)
-: SE.Steel byte_array
+  (#base: Type)
+  (a: byte_array base)
+: SE.Steel (byte_array base)
     (vparse (p1 `nondep_then` p2) a)
     (fun res -> vparse p1 a `SE.star` vparse p2 res)
     (fun _ ->
@@ -83,14 +83,14 @@ val destruct_pair
     )
 
 let destruct_pair
-  #k1 #t1 #p1 j1 p2 a
+  #k1 #t1 #p1 j1 p2 #base a
 =
   elim_vparse (p1 `nondep_then` p2) a;
-  let b : Ghost.erased (AP.v byte) = SEA.gget (AP.varrayptr a) in
+  let b : Ghost.erased (AP.v base byte) = SEA.gget (AP.varrayptr a) in
   nondep_then_eq p1 p2 b.AP.contents;
   let res = peek_strong j1 a in
   SEA.reveal_star (vparse p1 a) (AP.varrayptr res);
-  let c1 : Ghost.erased (v k1 t1) = SEA.gget (vparse p1 a) in // FIXME: WHY WHY WHY is the type annotation needed?
+  let c1 : Ghost.erased (v base k1 t1) = SEA.gget (vparse p1 a) in // FIXME: WHY WHY WHY is the type annotation needed?
   parse_strong_prefix p1 (Seq.slice b.AP.contents 0 (A.length (array_of c1))) b.AP.contents;
   intro_vparse p2 res;
   SEA.return res
@@ -103,8 +103,9 @@ val construct_pair
   (#k2: parser_kind)
   (#t2: Type)
   (p2: parser k2 t2)
-  (a1: byte_array)
-  (a2: byte_array)
+  (#base: Type)
+  (a1: byte_array base)
+  (a2: byte_array base)
 : SEA.SteelGhost unit opened
     (vparse p1 a1 `SE.star` vparse p2 a2)
     (fun _ -> vparse (p1 `nondep_then` p2) a1)
@@ -124,15 +125,15 @@ val construct_pair
 #restart-solver
 
 let construct_pair
-  #opened #k1 #t1 p1 p2 a1 a2
+  #opened #k1 #t1 p1 p2 #base a1 a2
 =
-  let v1 : Ghost.erased (v k1 t1) = SEA.gget (vparse p1 a1) in // FIXME: WHY WHY WHY is this type annotation needed?
+  let v1 : Ghost.erased (v base k1 t1) = SEA.gget (vparse p1 a1) in // FIXME: WHY WHY WHY is this type annotation needed?
   elim_vparse p1 a1;
   elim_vparse p2 a2;
-  let g1 = SEA.gget (AP.varrayptr a1) in
-  let g2 = SEA.gget (AP.varrayptr a2) in
+  let g1 : Ghost.erased (AP.v base byte) = SEA.gget (AP.varrayptr a1) in
+  let g2 : Ghost.erased (AP.v base byte) = SEA.gget (AP.varrayptr a2) in
   AP.join a1 a2;
-  let g : Ghost.erased (AP.v byte) = SEA.gget (AP.varrayptr a1) in // FIXME: same here
+  let g : Ghost.erased (AP.v base byte) = SEA.gget (AP.varrayptr a1) in // FIXME: same here
   nondep_then_eq p1 p2 g.AP.contents;
   Seq.lemma_append_inj g1.AP.contents g2.AP.contents (Seq.slice g.AP.contents 0 (A.length (array_of v1))) (Seq.slice g.AP.contents (A.length (array_of v1)) (Seq.length g.AP.contents));
   parse_strong_prefix p1 g1.AP.contents g.AP.contents;
@@ -151,14 +152,14 @@ let size_pair
   (j2: parsed_size p2)
 : Tot (parsed_size (p1 `nondep_then` p2))
 =
-  fun a ->
-  let g : Ghost.erased (AP.v byte) = SEA.gget (AP.varrayptr a) in
+  fun base a ->
+  let g : Ghost.erased (AP.v base byte) = SEA.gget (AP.varrayptr a) in
   nondep_then_eq p1 p2 g.AP.contents;
-  let len1 = j1 a in
+  let len1 = j1 base a in
   let a2 = AP.split a len1 in
-  let len2 = j2 a2 in
+  let len2 = j2 base a2 in
   AP.join a a2;
-  SEA.return (len1 `U32.add` len2)
+  SEA.return (len1 `SZ.size_add` len2)
 
 val validate_synth
   (#k1: _) (#t1: _) (#p1: parser k1 t1) (v1: wvalidator p1)
@@ -168,16 +169,17 @@ val validate_synth
 
 let validate_synth
   #_ #_ #p1 v1 f2 _
-= fun a len ->
+= fun base a len ->
   Classical.forall_intro (Classical.move_requires (parse_synth_eq p1 f2));
-  v1 a len
+  v1 base a len
 
 val intro_vparse_synth
   (#opened: _)
   (#k1: _) (#t1: _) (p1: parser k1 t1)
   (#t2: _) (f2: (t1 -> GTot t2))
   (f2_inj: squash (synth_injective f2))
-  (a: byte_array)
+  (#base: _)
+  (a: byte_array base)
 : SEA.SteelGhost unit opened
     (vparse p1 a)
     (fun _ -> vparse (parse_synth p1 f2) a)
@@ -190,10 +192,10 @@ val intro_vparse_synth
     )
 
 let intro_vparse_synth
-  p1 f2 _ a
+  p1 f2 _ #base a
 =
   elim_vparse p1 a;
-  let g = SEA.gget (AP.varrayptr a) in
+  let g : Ghost.erased (AP.v base byte) = SEA.gget (AP.varrayptr a) in
   parse_synth_eq p1 f2 g.AP.contents;
   intro_vparse (parse_synth p1 f2) a
 
@@ -202,7 +204,8 @@ val elim_vparse_synth
   (#k1: _) (#t1: _) (p1: parser k1 t1)
   (#t2: _) (f2: (t1 -> GTot t2))
   (f2_inj: squash (synth_injective f2))
-  (a: byte_array)
+  (#base: _)
+  (a: byte_array base)
 : SEA.SteelGhost unit opened
     (vparse (parse_synth p1 f2) a)
     (fun _ -> vparse p1 a)
@@ -215,10 +218,10 @@ val elim_vparse_synth
     )
 
 let elim_vparse_synth
-  p1 f2 _ a
+  p1 f2 _ #base a
 =
   elim_vparse (parse_synth p1 f2) a;
-  let g = SEA.gget (AP.varrayptr a) in
+  let g : Ghost.erased (AP.v base byte) = SEA.gget (AP.varrayptr a) in
   parse_synth_eq p1 f2 g.AP.contents;
   intro_vparse p1 a
 
@@ -228,16 +231,17 @@ let size_synth
   (#t2: _) (f2: (t1 -> GTot t2))
   (f2_inj: squash (synth_injective f2))
 : Tot (parsed_size (p1 `parse_synth` f2))
-= fun a ->
-  let g = SEA.gget (AP.varrayptr a) in
+= fun base a ->
+  let g : Ghost.erased (AP.v base byte) = SEA.gget (AP.varrayptr a) in
   parse_synth_eq p1 f2 g.AP.contents;
-  j1 a
+  j1 base a
 
 val intro_vparse_filter
   (#opened: _)
   (#k: _) (#t: _) (p: parser k t)
   (f: (t -> GTot bool))
-  (a: byte_array)
+  (#base: _)
+  (a: byte_array base)
 : SEA.SteelGhost unit opened
     (vparse p a)
     (fun _ -> vparse (parse_filter p f) a)
@@ -251,10 +255,10 @@ val intro_vparse_filter
     )
 
 let intro_vparse_filter
-  p f a
+  p f #base a
 =
   elim_vparse p a;
-  let g = SEA.gget (AP.varrayptr a) in
+  let g : Ghost.erased (AP.v base byte) = SEA.gget (AP.varrayptr a) in
   parse_filter_eq p f g.AP.contents;
   intro_vparse (parse_filter p f) a
 
@@ -262,7 +266,8 @@ val elim_vparse_filter
   (#opened: _)
   (#k: _) (#t: _) (p: parser k t)
   (f: (t -> GTot bool))
-  (a: byte_array)
+  (#base: _)
+  (a: byte_array base)
 : SEA.SteelGhost unit opened
     (vparse (parse_filter p f) a)
     (fun _ -> vparse p a)
@@ -276,10 +281,10 @@ val elim_vparse_filter
     )
 
 let elim_vparse_filter
-  p f a
+  p f #base a
 =
   elim_vparse (parse_filter p f) a;
-  let g = SEA.gget (AP.varrayptr a) in
+  let g : Ghost.erased (AP.v base byte) = SEA.gget (AP.varrayptr a) in
   parse_filter_eq p f g.AP.contents;
   intro_vparse p a
 
@@ -288,11 +293,11 @@ let size_filter
   (j: parsed_size p)
   (f: (t -> GTot bool))
 : Tot (parsed_size (p `parse_filter` f))
-= fun a ->
-  let g = SEA.gget (AP.varrayptr a) in
+= fun base a ->
+  let g : Ghost.erased (AP.v base byte) = SEA.gget (AP.varrayptr a) in
   assert (Some? (parse (parse_filter p f) g.AP.contents)); // FIXME: WHY WHY WHY?
   parse_filter_eq p f g.AP.contents;
-  j a
+  j base a
 
 [@ CMacro ]
 let validator_error_constraint_failed : validator_error = normalize_term (set_validator_error_kind 0uL 6uL)
@@ -302,9 +307,10 @@ let test_filter
   (#t: Type)
   (p: parser k t)
   (f: (t -> GTot bool))
-: Tot Type0
+: Tot (Type u#1)
 = 
-    (x: byte_array) ->
+    (base: Type0) ->
+    (x: byte_array base) ->
     SE.Steel bool
     (vparse p x)
     (fun _ -> vparse p x)
@@ -327,22 +333,22 @@ val validate_filter_gen
 
 let validate_filter_gen
   #_ #_ #p v32 f f'
-= fun a len ->
-  let glong = SEA.gget (AP.varrayptr a) in
+= fun base a len ->
+  let glong : Ghost.erased (AP.v base byte) = SEA.gget (AP.varrayptr a) in
   parse_filter_eq p f glong.AP.contents;
-  let res = v32 a len in
+  let res = v32 base a len in
   if is_error res
   then SEA.return res
   else begin
     let rlen = uint64_to_uint32 res () in
-    let a2 = AP.split a rlen in
-    let gshort = SEA.gget (AP.varrayptr a) in
+    let a2 = AP.split a (SZ.mk_size_t rlen) in
+    let gshort : Ghost.erased (AP.v base byte) = SEA.gget (AP.varrayptr a) in
     parse_strong_prefix p gshort.AP.contents glong.AP.contents;
     parse_filter_eq p f gshort.AP.contents;
     intro_vparse p a;
-    let v = f' a in
+    let v = f' base a in
     elim_vparse p a;
-    let gshort' = SEA.gget (AP.varrayptr a) in
+    let gshort' : Ghost.erased (AP.v base byte) = SEA.gget (AP.varrayptr a) in
     AP.join a a2;
     parse_injective p gshort.AP.contents gshort'.AP.contents; // because of the intro_vparse ; elim_vparse sequence
     if v
@@ -365,7 +371,7 @@ val validate_filter
 let validate_filter
   #_ #_ #p v32 p32 f f'
 = validate_filter_gen v32 f
-    (fun a -> let r = p32 a in SEA.return (f' r))
+    (fun base a -> let r = p32 base a in SEA.return (f' r))
 
 val validate_filter'
   (#k: parser_kind)
