src/lowparse/LowParse.Steel.VParse.fst
@@ -4,7 +4,7 @@ include LowParse.Spec.Base
 module S = Steel.Memory
 module SE = Steel.Effect
 module SEA = Steel.Effect.Atomic
-module A = Steel.Array
+module A = Steel.C.Array
 module AP = LowParse.Steel.ArrayPtr
 
 let is_byte_repr_injective
@@ -12,68 +12,74 @@ let is_byte_repr_injective
 = parse_injective p b1 b2
 
 let cvalid
+  (#base: Type)
   (#k: parser_kind)
   (#t: Type)
   (p: parser k t)
-  (c: AP.v byte)
+  (c: AP.v base byte)
 : Tot prop
 = valid p c.AP.contents /\
   array_prop k c.AP.array
 
 unfold
 let intro_cvalid
-  (a: byte_array)
+  (#base: Type)
+  (a: byte_array base)
   (#k: parser_kind)
   (#t: Type)
   (p: parser k t)
-  (c: AP.v byte)
+  (c: AP.v base byte)
   (sq: squash (cvalid p c))
 : Tot (SE.t_of (AP.varrayptr a `SE.vrefine` cvalid p))
 = c
 
 let select
-  (a: byte_array)
+  (#base: Type)
+  (a: byte_array base)
   (#k: parser_kind)
   (#t: Type)
   (p: parser k t)
   (x: SE.t_of (AP.varrayptr a `SE.vrefine` cvalid p))
-: GTot (v k t)
+: GTot (v base k t)
 =
-  let x : AP.v byte = x in
+  let x : AP.v base byte = x in
   let Some (y, _) = parse p x.AP.contents in
   {
-    array_perm = (x.AP.array, x.AP.perm);
+    array_perm = (x.AP.array); // , x.AP.perm);
     contents = y;
     array_perm_prf = ();
   }
 
 let select_correct
-  (a: byte_array)
+  (#base: Type)
+  (a: byte_array base)
   (#k: parser_kind)
   (#t: Type)
   (p: parser k t)
-  (x: SE.t_of (AP.varrayptr a `SE.vrefine` cvalid p))
+  (x: SE.normal (SE.t_of (AP.varrayptr a `SE.vrefine` cvalid p)))
 : Lemma
   (is_byte_repr p (select a p x).contents x.AP.contents)
 = ()
 
 let vparse0
+  (#base: Type)
   (#k: parser_kind)
   (#t: Type)
   (p: parser k t)
-  (a: byte_array)
+  (a: byte_array base)
 : Pure SE.vprop
   (requires True)
-  (ensures (fun y -> SE.t_of y == v k t))
+  (ensures (fun y -> SE.t_of y == v base k t))
 = (AP.varrayptr a `SE.vrefine` cvalid p) `SE.vrewrite`  select a p
 
 unfold
 let vparse0_sel
   (#p:SE.vprop)
+  (#base: Type)
   (#k: parser_kind) (#t: Type) (q: parser k t)
-  (r:byte_array)
+  (r:byte_array base)
   (h:SE.rmem p{FStar.Tactics.with_tactic SE.selector_tactic (SE.can_be_split p (vparse0 q r) /\ True)})
-: GTot (v k t)
+: GTot (v base k t)
 = let x : (SE.t_of (vparse0 q r)) =
     h (vparse0 q r)
   in
@@ -81,10 +87,11 @@ let vparse0_sel
 
 let intro_vparse0
   (#opened: _)
+  (#base: Type)
   (#k: parser_kind)
   (#t: Type)
   (p: parser k t)
-  (a: byte_array)
+  (a: byte_array base)
 : SEA.SteelGhost unit opened
     (AP.varrayptr a)
     (fun _ -> vparse0 p a)
@@ -93,7 +100,7 @@ let intro_vparse0
     )
     (fun h _ h' ->
       valid p (h (AP.varrayptr a)).AP.contents /\
-      perm_of (vparse0_sel p a h') == (h (AP.varrayptr a)).AP.perm /\
+//      perm_of (vparse0_sel p a h') == (h (AP.varrayptr a)).AP.perm /\
       array_of (vparse0_sel p a h') == (h (AP.varrayptr a)).AP.array /\
       is_byte_repr p (vparse0_sel p a h').contents (h (AP.varrayptr a)).AP.contents
     )
@@ -111,63 +118,65 @@ let change_equal_slprop (#opened: _) (p q: SE.vprop)
 
 let elim_vparse0
   (#opened: _)
+  (#base: Type)
   (#k: parser_kind)
   (#t: Type)
   (p: parser k t)
-  (a: byte_array)
+  (a: byte_array base)
 : SEA.SteelGhost unit opened
     (vparse0 p a)
     (fun _ -> AP.varrayptr a)
     (fun _ -> True)
     (fun h _ h' ->
       (h' (AP.varrayptr a)).AP.array == array_of (vparse0_sel p a h) /\
-      (h' (AP.varrayptr a)).AP.perm == perm_of (vparse0_sel p a h) /\
+//      (h' (AP.varrayptr a)).AP.perm == perm_of (vparse0_sel p a h) /\
       valid p (h' (AP.varrayptr a)).AP.contents /\
       is_byte_repr p (vparse0_sel p a h).contents (h' (AP.varrayptr a)).AP.contents
     )
 =
-  let sq : squash (vparse0 #k #t p a == (AP.varrayptr a `SE.vrefine` cvalid p) `SE.vrewrite` select a p) =
-    assert_norm (vparse0 #k #t p a == (AP.varrayptr a `SE.vrefine` cvalid p) `SE.vrewrite` select a p)
+  let sq : squash (vparse0 #base #k #t p a == (AP.varrayptr a `SE.vrefine` cvalid p) `SE.vrewrite` select a p) =
+    assert_norm (vparse0 #base #k #t p a == (AP.varrayptr a `SE.vrefine` cvalid p) `SE.vrewrite` select a p)
   in
-  change_equal_slprop (vparse0 #k #t p a)
+  change_equal_slprop (vparse0 #base #k #t p a)
     ((AP.varrayptr a `SE.vrefine` cvalid p) `SE.vrewrite` select a p)
     sq;
   SEA.elim_vrewrite (AP.varrayptr a `SE.vrefine` cvalid p) (select a p);
   let g = SEA.gget (AP.varrayptr a `SE.vrefine` cvalid p) in
-  assert (valid p (Ghost.reveal g).AP.contents);
+  assert (valid p (Ghost.reveal g <: AP.v base byte).AP.contents);
   SEA.elim_vrefine (AP.varrayptr a) (cvalid p)
 
 let vparse_slprop
-  #k #t p a
+  #base #k #t p a
 =
-  SE.hp_of (vparse0 #k #t p a)
+  SE.hp_of (vparse0 #base #k #t p a)
 
 let vparse_sel
-  #k #t p a
+  p a
 =
-  fun m -> SE.sel_of (vparse0 p a) m
+  SE.sel_of (vparse0 p a)
 
 let intro_vparse
-  #opened #k #t p a
+  #opened #base #k #t p a
 =
   intro_vparse0 p a;
   SEA.change_slprop_rel
     (vparse0 p a)
     (vparse p a)
-    (fun (x: SE.t_of (vparse0 p a)) (y: SE.t_of (vparse p a)) -> (x <: v k t) == y)
+    (fun (x: SE.t_of (vparse0 p a)) (y: SE.t_of (vparse p a)) -> (x <: v base k t) == y)
     (fun _ -> ());
   ()
 
 let elim_vparse
-  #opened #k #t p a
+  #opened #base #k #t p a
 =
   SEA.change_slprop_rel
     (vparse p a)
     (vparse0 p a)
-    (fun (x: SE.t_of (vparse p a)) (y: SE.t_of (vparse0 p a)) -> (x <: v k t) == y)
+    (fun (x: SE.t_of (vparse p a)) (y: SE.t_of (vparse0 p a)) -> (x <: v base k t) == y)
     (fun _ -> ());
   elim_vparse0 p a
 
+(*
 let share
   p a
 =
@@ -186,3 +195,4 @@ let gather
   elim_vparse p a2;
   AP.gather a1 a2;
   intro_vparse p a1
+*)
