src/lowparse/LowParse.Steel.VParse.fsti
@@ -5,12 +5,12 @@ module S = Steel.Memory
 module SP = Steel.FractionalPermission
 module SE = Steel.Effect
 module SEA = Steel.Effect.Atomic
-module A = Steel.Array
+module A = Steel.C.Array
 module AP = LowParse.Steel.ArrayPtr
 
 (* For now, we only support parsers with ParserStrong or ParserConsumesAll subkind. *)
 
-let byte_array : Type0 = AP.t byte
+let byte_array (base: Type0) : Type0 = AP.t base byte
 
 let valid
   (#k: parser_kind)
@@ -48,90 +48,98 @@ val is_byte_repr_injective
   (requires (is_byte_repr p x b1 /\ is_byte_repr p x b2))
   (ensures (b1 == b2))
 
-let array_prop (k: parser_kind) (a: A.array byte) : Tot prop =
+let array_prop (#base: Type) (k: parser_kind) (a: A.array base byte) : Tot prop =
   let l = A.length a in
   k.parser_kind_low <= l /\
   (Some? k.parser_kind_high ==> l <= Some?.v k.parser_kind_high)
 
-let array_t (k: parser_kind) : Tot Type =
-  (array: A.array byte { array_prop k array })
+let array_t (base: Type) (k: parser_kind) : Tot Type =
+  (array: A.array base byte { array_prop k array })
 
 [@@erasable]
 noeq
-type v (k: parser_kind) (t: Type) = {
-  array_perm : (A.array byte & SP.perm);
+type v (base: Type) (k: parser_kind) (t: Type) = {
+  array_perm : (A.array base byte); // & SP.perm);
   contents : t;
-  array_perm_prf: squash (array_prop k (fst array_perm));
+  array_perm_prf: squash (array_prop k ((* fst *) array_perm));
 }
 
-let array_of (#k: parser_kind) (#t: Type) (w: v k t) : GTot (array_t k) =
-  fst w.array_perm
+let array_of (#base: Type) (#k: parser_kind) (#t: Type) (w: v base k t) : GTot (array_t base k) =
+//  fst
+  w.array_perm
 
-let perm_of (#k: parser_kind) (#t: Type) (w: v k t) : Tot SP.perm =
-  snd w.array_perm
+// let perm_of (#base: Type) (#k: parser_kind) (#t: Type) (w: v base k t) : Tot SP.perm =
+//  snd w.array_perm
 
 let adjacent
+  (#base: Type)
   (#t1 #t2: Type)
   (#k1 #k2: parser_kind)
-  (v1: v k1 t1)
-  (v2: v k2 t2)
+  (v1: v base k1 t1)
+  (v2: v base k2 t2)
 : Tot prop
 = A.adjacent (array_of v1) (array_of v2) /\
-  perm_of v1 == perm_of v2
+  True //  perm_of v1 == perm_of v2
 
 let merge_into
+  (#base: Type)
   (#k1 #k2 #k: parser_kind)
   (#t1 #t2 #t: Type)
-  (v1: v k1 t1)
-  (v2: v k2 t2)
-  (v: v k t)
+  (v1: v base k1 t1)
+  (v2: v base k2 t2)
+  (v: v base k t)
 : Tot prop
 = A.merge_into (array_of v1) (array_of v2) (array_of v) /\
-  perm_of v1 == perm_of v /\
-  perm_of v2 == perm_of v
+True //  perm_of v1 == perm_of v /\
+//  perm_of v2 == perm_of v
 
 val vparse_slprop
+  (#base: Type)
   (#k: parser_kind)
   (#t: Type0)
   (p: parser k t)
-  (a: byte_array)
+  (a: byte_array base)
 : Tot (S.slprop u#1)
 
 val vparse_sel
+  (#base: Type)
   (#k: parser_kind)
   (#t: Type)
   (p: parser k t)
-  (a: byte_array)
-: Tot (SE.selector (v k t) (vparse_slprop p a))
+  (a: byte_array base)
+: GTot (SE.selector (v base k t) (vparse_slprop p a))
 
 [@SE.__steel_reduce__]
 let vparse'
+  (#base: Type)
   (#k: parser_kind)
   (#t: Type)
   (p: parser k t)
-  (a: byte_array)
+  (a: byte_array base)
 : Tot SE.vprop'
 = {
   SE.hp = vparse_slprop p a;
-  SE.t = v k t;
+  SE.t = v base k t;
   SE.sel = vparse_sel p a;
 }
 
 [@SE.__steel_reduce__]
 let vparse
+  (#base: Type)
   (#k: parser_kind)
   (#t: Type)
   (p: parser k t)
-  (a: byte_array)
+  (a: byte_array base)
 : Tot SE.vprop
 = SE.VUnit (vparse' p a)
 
 val intro_vparse
   (#opened: _)
+  (#base: Type)
   (#k: parser_kind)
   (#t: Type)
   (p: parser k t)
-  (a: byte_array)
+  (a: byte_array base)
 : SEA.SteelGhost unit opened
     (AP.varrayptr a)
     (fun _ -> vparse p a)
@@ -143,16 +151,17 @@ val intro_vparse
       let s = h (AP.varrayptr a) in
       valid p s.AP.contents /\
       array_of s' == s.AP.array /\
-      perm_of s' == s.AP.perm /\
+//      perm_of s' == s.AP.perm /\
       is_byte_repr p s'.contents s.AP.contents
     )
 
 val elim_vparse
   (#opened: _)
+  (#base: Type)
   (#k: parser_kind)
   (#t: Type)
   (p: parser k t)
-  (a: byte_array)
+  (a: byte_array base)
 : SEA.SteelGhost unit opened
     (vparse p a)
     (fun _ -> AP.varrayptr a)
@@ -161,18 +170,20 @@ val elim_vparse
       let s' = h' (AP.varrayptr a) in
       let s = h (vparse p a) in
       valid p s'.AP.contents /\
-      s'.AP.perm == perm_of s /\
+//      s'.AP.perm == perm_of s /\
       s'.AP.array == array_of s /\
       is_byte_repr p s.contents s'.AP.contents
     )
 
+(*
 val share
   (#opened: _)
+  (#base: Type)
   (#k: parser_kind)
   (#t: Type)
   (p: parser k t)
-  (a: byte_array)
-: SEA.SteelAtomic byte_array opened
+  (a: byte_array base)
+: SEA.SteelAtomic (byte_array base) opened
     (vparse p a)
     (fun res -> vparse p a `SE.star` vparse p res)
     (fun _ -> True)
@@ -181,19 +192,20 @@ val share
       let s' = h' (vparse p a) in
       let d = h' (vparse p res) in
       array_of s' == array_of s /\
-      perm_of s' == SP.half_perm (perm_of s) /\
+//      perm_of s' == SP.half_perm (perm_of s) /\
       s'.contents == s.contents /\
       array_of d == array_of s /\
-      perm_of d == SP.half_perm (perm_of s) /\
+//      perm_of d == SP.half_perm (perm_of s) /\
       d.contents == s.contents
     )
 
 val gather
   (#opened: _)
+  (#base: Type)
   (#k: parser_kind)
   (#t: Type)
   (p: parser k t)
-  (a1 a2: byte_array)
+  (a1 a2: byte_array base)
 : SEA.SteelGhost unit opened
     (vparse p a1 `SE.star` vparse p a2)
     (fun res -> vparse p a1)
@@ -206,7 +218,8 @@ val gather
       let d = h' (vparse p a1) in
       array_of d == array_of s1 /\
       array_of d == array_of s2 /\
-      perm_of d == perm_of s1 `SP.sum_perm` perm_of s2 /\
+//      perm_of d == perm_of s1 `SP.sum_perm` perm_of s2 /\
       d.contents == s1.contents /\
       d.contents == s2.contents
     )
+*)
