src/lowparse/LowParse.Steel.Validate.fst
@@ -5,9 +5,10 @@ include LowParse.Low.ErrorCode
 module S = Steel.Memory
 module SE = Steel.Effect
 module SEA = Steel.Effect.Atomic
-module A = Steel.Array
+module A = Steel.C.Array
 module AP = LowParse.Steel.ArrayPtr
 
+module SZ = Steel.C.StdInt
 module U32 = FStar.UInt32
 module U64 = FStar.UInt64
 
@@ -16,10 +17,11 @@ module U64 = FStar.UInt64
    those marked ConsumesAll. *)
 
 let tvalid_res_vprop
+  (#base: Type)
   (#t: Type0)
   (#k: parser_kind)
   (p: parser k t)
-  (a: byte_array)
+  (a: byte_array base)
   (res: bool)
 : Tot SE.vprop
 = if res
@@ -28,26 +30,28 @@ let tvalid_res_vprop
 
 unfold
 let tvalid_res_vprop_true
+  (#base: Type)
   (#t: Type0)
   (#k: parser_kind)
   (p: parser k t)
-  (a: byte_array)
+  (a: byte_array base)
   (res: bool)
   (x: SE.t_of (tvalid_res_vprop p a res))
-: Pure (v k t)
+: Pure (v base k t)
   (requires (res == true))
   (ensures (fun _ -> True))
 = x
 
 unfold
 let tvalid_res_vprop_false
+  (#base: Type)
   (#t: Type0)
   (#k: parser_kind)
   (p: parser k t)
-  (a: byte_array)
+  (a: byte_array base)
   (res: bool)
   (x: SE.t_of (tvalid_res_vprop p a res))
-: Pure (AP.v byte)
+: Pure (AP.v base byte)
   (requires (res == false))
   (ensures (fun _ -> True))
 = x
@@ -58,7 +62,8 @@ let tvalidator
   (p: parser k t)
 : Tot Type
 =
-  (a: byte_array) ->
+  (base: Type0) ->
+  (a: byte_array base) ->
   (len: U32.t) ->
   SE.Steel bool
     (AP.varrayptr a)
@@ -72,7 +77,7 @@ let tvalidator
       then
         let s' = tvalid_res_vprop_true p a res s' in
         array_of s' == s.AP.array /\
-        perm_of s' == s.AP.perm /\
+//        perm_of s' == s.AP.perm /\
         is_byte_repr p s'.contents s.AP.contents
       else
         let s' = tvalid_res_vprop_false p a res s' in
@@ -93,7 +98,8 @@ let wvalidator
   (p: parser k t)
 : Tot Type
 =
-  (a: byte_array) ->
+  (base: Type) ->
+  (a: byte_array base) ->
   (len: U32.t) ->
   SE.Steel U64.t
     (AP.varrayptr a)
@@ -112,15 +118,16 @@ let wvalidator
     )
 
 let wvalidate_post // FIXME: WHY WHY WHY do I need to define this postcondition separately? (if not, then dummy fails to verify)
+  (#base: Type)
   (#t: Type0)
   (#k: parser_kind)
   (p: parser k t)
-  (a: byte_array)
+  (a: byte_array base)
   (len: U32.t)
-  (res: byte_array)
-  (s: AP.v byte)
+  (res: byte_array base)
+  (s: AP.v base byte)
   (s': SE.t_of (if AP.g_is_null res then AP.varrayptr a else vparse p a))
-  (vres: option (AP.v byte))
+  (vres: option (AP.v base byte))
 : Tot prop
 =
   if AP.g_is_null res
@@ -129,12 +136,12 @@ let wvalidate_post // FIXME: WHY WHY WHY do I need to define this postcondition 
     vres == None /\
     s' == s
   else begin
-    let s' : v k t = s' in
+    let s' : v base k t = s' in
     let consumed = A.length (array_of s') in
     Some? vres /\
     U32.v len == A.length s.AP.array /\
-    perm_of s' == s.AP.perm /\
-    (Some?.v vres).AP.perm == s.AP.perm /\
+//    perm_of s' == s.AP.perm /\
+//    (Some?.v vres).AP.perm == s.AP.perm /\
     A.merge_into (array_of s') (Some?.v vres).AP.array s.AP.array /\
     consumed <= A.length s.AP.array /\
     is_byte_repr p s'.contents (Seq.slice s.AP.contents 0 consumed) /\
@@ -142,13 +149,14 @@ let wvalidate_post // FIXME: WHY WHY WHY do I need to define this postcondition 
   end
 
 val wvalidate
+  (#base: Type)
   (#t: Type0)
   (#k: parser_kind)
   (#p: parser k t)
   (w: wvalidator p)
-  (a: byte_array)
+  (a: byte_array base)
   (len: U32.t)
-: SE.Steel (byte_array)
+: SE.Steel (byte_array base)
     (AP.varrayptr a)
     (fun res -> (if AP.g_is_null res then AP.varrayptr a else vparse p a) `SE.star` AP.varrayptr_or_null res)
     (fun h -> U32.v len == A.length (h (AP.varrayptr a)).AP.array)
@@ -160,12 +168,12 @@ val wvalidate
     )
 
 let wvalidate
-  #t #k #p w a len
+  #base #t #k #p w a len
 =
-  let consumed = w a len in
+  let consumed = w base a len in
   if is_success consumed
   then begin
-    let ar : byte_array = AP.split a (uint64_to_uint32 consumed) in
+    let ar : byte_array base = AP.split a (SZ.mk_size_t (uint64_to_uint32 consumed)) in
     intro_vparse p a;
     AP.intro_varrayptr_or_null_some ar;
     SEA.change_equal_slprop
@@ -173,7 +181,7 @@ let wvalidate
       (if AP.g_is_null ar then AP.varrayptr a else vparse p a);
     SEA.return ar
   end else begin
-    let res : byte_array = AP.null _ in
+    let res : byte_array base = AP.null _ _ in
     AP.intro_varrayptr_or_null_none res;
     SEA.change_equal_slprop
       (AP.varrayptr a)
@@ -182,11 +190,12 @@ let wvalidate
   end
 
 let dummy
+  (#base: Type)
   (#t: Type0)
   (#k: parser_kind)
   (#p: parser k t)
   (w: wvalidator p)
-  (a: byte_array)
+  (a: byte_array base)
   (len: U32.t)
 : SE.Steel unit
     (AP.varrayptr a)
@@ -196,7 +205,7 @@ let dummy
       h' (AP.varrayptr a) == h (AP.varrayptr a)
     )
 =
-  let g0 : Ghost.erased (AP.v byte) = SEA.gget (AP.varrayptr a) in
+  let g0 : Ghost.erased (AP.v base byte) = SEA.gget (AP.varrayptr a) in
   let res = wvalidate w a len in
   if AP.is_null res
   then begin
@@ -210,9 +219,9 @@ let dummy
       (if AP.g_is_null res then AP.varrayptr a else vparse p a)
       (vparse p a);
     AP.elim_varrayptr_or_null_some res;
-    let g1 : Ghost.erased (v k t) = SEA.gget (vparse p a) in // FIXME: WHY WHY WHY is this type annotation needed?
+    let g1 : Ghost.erased (v base k t) = SEA.gget (vparse p a) in // FIXME: WHY WHY WHY is this type annotation needed?
     elim_vparse p a;
-    let g2 = SEA.gget (AP.varrayptr a) in
+    let g2 : Ghost.erased (AP.v base byte) = SEA.gget (AP.varrayptr a) in
     let glen = Ghost.hide (A.length (array_of (Ghost.reveal g1))) in
     is_byte_repr_injective p (Ghost.reveal g1).contents (Seq.slice (Ghost.reveal g0).AP.contents 0 (Ghost.reveal glen)) (Ghost.reveal g2).AP.contents;
     Seq.lemma_split (Ghost.reveal g0).AP.contents (Ghost.reveal glen);
@@ -267,9 +276,9 @@ let validate_total_constant_size
         k.parser_kind_low == U32.v sz
     ))
     (ensures (fun _ -> True))
-= fun (a: byte_array) (len: U32.t) ->
+= fun base (a: byte_array base) (len: U32.t) ->
   let ga = SEA.gget (AP.varrayptr a) in
-  let g = Ghost.hide (Ghost.reveal ga).AP.contents in
+  let g = Ghost.hide (Ghost.reveal ga <: AP.v base byte).AP.contents in
   parser_kind_prop_equiv k p;
   if len `U32.lt` sz
   then begin
