src/lowparse/LowParse.Steel.Leaf.fst
@@ -7,15 +7,17 @@ module SP = Steel.FractionalPermission
 module S = Steel.Memory
 module SE = Steel.Effect
 module SEA = Steel.Effect.Atomic
-module A = Steel.Array
+module A = Steel.C.Array
 module AP = LowParse.Steel.ArrayPtr
 
 let leaf_reader
   (#k: parser_kind)
   (#t: Type)
   (p: parser k t)
-: Tot Type0
-= (src: byte_array) ->
+: Tot (Type u#1)
+=
+  (base: Type) ->
+  (src: byte_array base) ->
   SE.Steel t
     (vparse p src)
     (fun _ -> vparse p src)
@@ -28,48 +30,51 @@ let leaf_reader
 
 let exact_serializer
   (#k: parser_kind)
-  (#t: Type)
+  (#t: Type0)
   (#p: parser k t)
   (s: serializer p)
-: Tot Type0
-= (dst: byte_array) ->
+: Tot (Type u#1)
+=
+  (base: Type0) ->
+  (dst: byte_array base) ->
   (x: t) ->
   SE.Steel unit
     (AP.varrayptr dst)
     (fun _ -> AP.varrayptr dst)
     (requires (fun h ->
       A.length (h (AP.varrayptr dst)).AP.array == Seq.length (serialize s x) /\
-      (h (AP.varrayptr dst)).AP.perm == SP.full_perm
+True //      (h (AP.varrayptr dst)).AP.perm == SP.full_perm
     ))
     (ensures (fun h _ h' ->
       let d = h (AP.varrayptr dst) in
       let d' = h' (AP.varrayptr dst) in
       d'.AP.array == d.AP.array /\
-      d'.AP.perm == d.AP.perm /\
+//      d'.AP.perm == d.AP.perm /\
       d'.AP.contents == serialize s x
     ))
 
 let write_exact
+  (#base: Type)
   (#k: parser_kind)
-  (#t: Type)
+  (#t: Type0)
   (#p: parser k t)
   (#s: serializer p)
   (w: exact_serializer s)
-  (dst: byte_array)
+  (dst: byte_array base)
   (x: t)
 : SE.Steel unit
     (AP.varrayptr dst)
     (fun _ -> vparse p dst)
     (requires (fun h ->
       A.length (h (AP.varrayptr dst)).AP.array == Seq.length (serialize s x) /\
-      (h (AP.varrayptr dst)).AP.perm == SP.full_perm
+True //      (h (AP.varrayptr dst)).AP.perm == SP.full_perm
     ))
     (ensures (fun h _ h' ->
       let d = h (AP.varrayptr dst) in
       let d' = h' (vparse p dst) in
       array_of d' == d.AP.array /\
-      perm_of d' == SP.full_perm /\
+//      perm_of d' == SP.full_perm /\
       d'.contents == x
     ))
-= w dst x;
+= w _ dst x;
   intro_vparse p dst
